Makefile
@@ -1,7 +1,15 @@
 MY_FSTAR_HOME=`cygpath "$(FSTAR_HOME)"`
 
-all: SamlProtocol
+all: samlProtocol
 
-SamlProtocol:
+samlProtocol:
 	mkdir -p bin
-	fstar --genIL --writePrims --odir bin --dotnet4 simplecrypto.fst
+	fstar --genIL --writePrims --odir bin --dotnet4 --parallel samlProtocol.fst
+
+crypto:
+	mkdir -p bin
+	fstar --genIL --writePrims --odir bin --dotnet4 --parallel simplecrypto.fst
+
+
+clean:
+	rm -rf bin
